src/LibListZ.v
@@ -1,5 +1,3 @@
-(*--TODO COMPLETE CLEANUP --*)
-
 (**************************************************************************
 * TLC: A library for Coq                                                  *
 * Lists accessed with integers (not nat), using LibContainer typeclasses  *
@@ -42,10 +40,10 @@ Proof using. auto. Qed.
 Lemma abs_length : forall i l,
   i = length l ->
   abs i = LibList.length l.
-Proof using. (* --TODO: cleanup proof *)
-  unfold length. intros. subst.
-  generalize (LibList.length l). clear A l. (* for clarity *)
-  rew_maths. eapply Zabs2Nat.id.
+Proof using.
+  introv E. unfold length in E.
+  applys eq_nat_of_eq_int.
+  rewrite abs_nonneg; math.
 Qed.
 
 Lemma length_nonneg : forall (l: list A), 
@@ -77,37 +75,16 @@ Lemma length_zero_inv : forall l,
   l = nil.
 Proof using. intros. unfolds length. applys~ LibList.length_zero_inv. Qed.
 
-(*-- TODO: there is no lemmas about [tail] in LibList;
-     should we keep these? *)
-(*
-Lemma length_tail : forall l,
-  l <> nil -> 
-  length (tail l) = length l - 1.
-Proof using. induction l; intros; simpl; unfold length; rew_list. congruence. math. Qed.
-
-Lemma length_tail_le : forall l,
-  length (tail l) <= length l.
-Proof using. destruct l; simpl; unfold length; rew_list; math. Qed.
-
-Lemma length_le_1_inv_tail_eq_nil : forall l,
-  length l <= 1 -> 
-  tail l = nil.
-Proof using.
-  intros. destruct l; eauto.
-  simpl. unfold length in *. rew_list in *.
-  eapply length_zero_inv. math.
-Qed.
-*)
-
 End Length.
 
 Hint Rewrite length_nil length_cons length_app
  length_last length_rev : rew_list.
- (* --TODO: should we use a separate [rew_listZ] data base ? *)
+ (* --TODO: should we use a separate [rew_listZ] data base? probably so *)
 
 (** Automation for [math], to unfold [length] *)
 
 Hint Rewrite length_eq : rew_maths.
+
 
 (** Demo of automation with maths *)
 
@@ -192,13 +169,13 @@ Proof using.
       case_if. math. auto. } }
 Qed.
 
-Lemma read_cons_zero : forall x l,
+Lemma read_zero : forall x l,
   (x::l)[0] = x.
 Proof using. 
   intros. rewrite read_cons_case. case_if. auto. 
 Qed.
 
-Lemma read_cons_succ : forall x l i,
+Lemma read_succ : forall x l i,
   0 <= i < length l ->
   (x::l)[i+1] = l[i].
 Proof using.
@@ -206,10 +183,8 @@ Proof using.
   fequals. math.
 Qed.
 
-(*--TODO: unclear if next lemma should be using [length] of [LibList.length] *)
-
 Lemma read_last_case : forall l i v,
-  (l & v)[i] = (If i = LibList.length l then v else l[i]).
+  (l & v)[i] = (If i = length l then v else l[i]).
 Proof using.
   introv. simpl. unfold read_impl. case_if.
   { case_if~; math. } 
@@ -237,39 +212,30 @@ Proof using.
   { applys ge_nat_of_ge_int. rewrite abs_nonneg; math. }
 Qed.
 
-End Read.
-
-Global Opaque read_inst.
-
-
-(* ---------------------------------------------------------------------- *)
 (** * Equality between two lists from equality of length and 
       extensional equality of reads. *)
 
-Lemma eq_of_extensional : forall `{Inhab A} (l1 l2:list A),
+Lemma eq_of_extens_range : forall l1 l2,
   length l1 = length l2 ->
   (forall i, 0 <= i < length l1 -> l1[i] = l2[i]) ->
   l1 = l2.
-Proof using. (* --LATER: cleanup proof *)
-  induction l1; destruct l2; simpl; introv Heq Hread;
-  try solve [ eauto | false ]. f_equal.
-  { specializes Hread 0.
-    repeat rewrite read_cons_zero in Hread.
-    repeat rewrite length_cons in Hread.
-    eapply Hread.
-    forwards: length_nonneg l1. math. }
-  { repeat rewrite length_cons in *.
-    eapply IHl1. math. intros i Hi.
-    specializes Hread (i + 1).
-    do 2 rewrite read_cons_succ in Hread by math.
-    eapply Hread. math. }
+Proof using.
+  introv HL HR. do 2 rewrite length_eq in HL.
+  unfold read, read_inst, read_impl in HR.
+  applys~ LibList.eq_of_extens l1 l2.
+  { intros n L. forwards M: (rm HR) (nat_to_Z n). math.
+    case_if. false; math. rewrite~ abs_nat in M. }
 Qed.
 
-Lemma eq_of_extensional_index : forall `{Inhab A} (l1 l2:list A),
+Lemma eq_of_extens : forall l1 l2,
   length l1 = length l2 ->
   (forall i, index l1 i -> l1[i] = l2[i]) ->
   l1 = l2.
-Proof using. intros. applys~ eq_of_extensional. Qed.
+Proof using. intros. applys~ eq_of_extens_range. Qed.
+
+End Read.
+
+Global Opaque read_inst.
 
 
 (* ---------------------------------------------------------------------- *)
@@ -281,10 +247,6 @@ Definition update_impl A (l:list A) (i:int) (v:A) : list A :=
 Instance update_inst : forall A, BagUpdate int A (list A).
 Proof using. constructor. rapply (@update_impl A). Defined.
 
-
-Notation "m [ x := v ]" := (LibContainer.update m x v)
-  (at level 9, format "m [ x := v ]", left associativity) :foo.
-
 Section Update.
 Transparent index_inst read_inst update_inst.
 Context (A : Type) `{IA:Inhab A}.
@@ -292,16 +254,12 @@ Implicit Types x v w : A.
 Implicit Types l : list A.
 Implicit Types i j : int.
 
-
-
-
 Lemma length_update : forall l i v,
   length (l[i:=v]) = length l.
 Proof using.
   intros. unfold update_inst, update_impl, length, update. simpl.
   case_if. math. rewrite~ length_update.
 Qed.
-
 
 Lemma index_update_eq : forall l i j v,
   index (l[j:=v]) i = index l i.
@@ -338,8 +296,6 @@ Proof using. introv N. rewrite~ read_update_case. case_if; auto_false~. Qed.
 
 End Update.
 
-
-
 Section UpdateNoInhab.
 Transparent index_inst read_inst update_inst.
 Context (A : Type).
@@ -347,18 +303,33 @@ Implicit Types x v w : A.
 Implicit Types l : list A.
 Implicit Types i j : int.
 
+Lemma update_zero : forall v x l,
+  (x::l)[0:=v] = v::l.
+Proof using. 
+  intros. unfold update, update_inst, update_impl.
+  case_if. false; math. rewrite~ update_zero.
+Qed.
+
+Lemma update_cons_pos : forall n v x l,
+  n > 0 ->
+  (x::l)[n:=v] = x::(l[(n-1):=v]).
+Proof using. 
+  introv N. unfold update, update_inst, update_impl.
+  do 2 (case_if; try solve [ false; math ]).
+  rewrite~ update_cons_pos. 
+  { fequals_rec. rewrite <- abs_gt_minus_nat. fequals. math. }
+  { applys gt_nat_of_gt_int. rewrite abs_nonneg; math. }
+Qed.
+
 Lemma update_update_same : forall l i v w,
   index l i ->
   l[i:=v][i:=w] = l[i:=w].
-Proof using. (* --TODO: cleanup proof *)
+Proof using. 
   intros. asserts IA: (Inhab A). typeclass.
-  eapply eq_of_extensional_index; repeat rewrite length_update.
-  { reflexivity. }
-  intros j.
-  repeat rewrite index_update_eq.
-  intros Hj.
+  eapply eq_of_extens; repeat rewrite length_update. { auto. }
+  intros k Hk. repeat rewrite index_update_eq in Hk.
   repeat rewrite read_update_case by eauto using index_update.
-  case_if; reflexivity.
+  case_if~.
 Qed.
 
 Lemma update_update_neq : forall l i j v w,
@@ -366,28 +337,33 @@ Lemma update_update_neq : forall l i j v w,
   index l j -> 
   i <> j -> 
   l[i:=v][j:=w] = l[j:=w][i:=v].
-Proof using. (* --TODO: cleanup proof *)
+Proof using.
   intros. asserts IA: (Inhab A). typeclass.
-  eapply eq_of_extensional_index; repeat rewrite length_update.
-  { reflexivity. }
-  intros k.
-  repeat rewrite index_update_eq.
-  intros Hk.
+  applys eq_of_extens; repeat rewrite length_update. { auto. }
+  intros k Hk. repeat rewrite index_update_eq in Hk.
   repeat rewrite read_update_case by eauto using index_update.
-  repeat case_if; reflexivity.
+  repeat case_if~.
 Qed.
 
-(*-- TODO: add lemma update_app_l *)
+Lemma update_app_l : forall l1 i l2 v,
+  0 <= i < length l1 ->
+  (l1 ++ l2)[i:=v] = (l1[i:=v]) ++ l2.
+Proof using.
+  introv N. asserts IA: (Inhab A). typeclass.
+  unfold LibContainer.update, update_inst, update_impl.
+  rewrite length_eq in N. case_if~. rewrite~ update_app_l. 
+  applys lt_nat_of_lt_int. rewrite~ abs_nonneg. 
+Qed.
 
 Lemma update_app_r : forall l2 j l1 i ij v,
   i = length l1 ->
   0 <= j ->
   ij = i + j ->
   (l1 ++ l2)[ij:=v] = l1 ++ (l2[j:=v]).
-Proof using. (* --TODO: cleanup proof *)
+Proof using.
   intros. asserts IA: (Inhab A). typeclass. subst ij.
   unfold LibContainer.update, update_inst, update_impl.
-  unfold update. do 2 (case_if; [ math | ]).
+  do 2 (case_if; [ math | ]).
   rewrite Zabs2Nat.inj_add; try math. subst i.
   rewrite length_eq. rewrite abs_nat.
   rewrite~ update_app_r. fequals_rec. math.
@@ -396,13 +372,9 @@ Qed.
 Lemma update_middle : forall i l1 l2 v w,
   i = length l1 ->
   (l1 ++ w :: l2)[i := v] = l1 & v ++ l2.
-Proof using. (* --TODO: cleanup proof *)
-  intros. asserts IA: (Inhab A). typeclass.
-  unfold LibContainer.update, update_inst, update_impl.
-  unfold update. case_if; [ math | ].
-  rewrite~ LibList.update_middle. subst i.
-  rewrite length_eq. rewrite~ abs_nat. 
-  (* -- LATER: factorize the pattern of the above line *)
+Proof using. 
+  introv E. rewrites~ (>> update_app_r 0 i).
+  rewrite update_zero. rew_list~.
 Qed.
 
 End UpdateNoInhab.
@@ -455,52 +427,68 @@ Qed.
 Lemma make_zero : forall v, 
   make 0 v = nil.
 Proof using.
-  intros. unfold make. case_if. { false; math. } 
-  asserts_rewrite (abs 0 = 0%nat). { applys eq_int_nat. rewrite abs_pos; math. }
+  intros. unfold make. case_if. { false; math. }
+  asserts_rewrite (abs 0 = 0%nat). 
+  { applys eq_nat_of_eq_int. rewrite abs_nonneg; math. }
   auto.
 Qed.
 
-Lemma make_succ_l: forall n v, 
+End Make.
+
+Section MakeNoInhab.
+Transparent index_inst read_inst.
+Context (A : Type).
+Implicit Types x v : A.
+Implicit Types l : list A.
+Implicit Types n i : int.
+
+Lemma make_succ_l : forall n v, 
   n >= 0 -> 
   make (n+1) v = v :: make n v.
 Proof using.
-  intros. rewrites <- (>> cons_make (n+1)). math. fequals_rec; math.
+  introv N. unfold make. case_if; case_if; try solve [false;math].
+  rewrite <- LibList.make_succ. fequal.
+  { rewrite succ_abs_eq_abs_one_plus. fequal. math. math. }
 Qed.
 
-Lemma make_succ_r: forall n v, 
+Lemma make_succ_r : forall n v, 
   n >= 0 -> 
   make (n+1) v = make n v & v.
 Proof using.
-  intros. asserts IA: (Inhab A). applys prove_Inhab x. applys ext_eq.
+  intros. asserts IA: (Inhab A). applys Inhab_of_val v.
+  applys eq_of_extens_range.
   { rewrite length_make. rew_list. rewrite length_make.
     math. math. math. }
   { intros i Ei. rewrite length_make in Ei; [| math ].
-    rewrite read_make; [| rewrite int_index_def; math ]. 
-    rewrite read_app. case_if as C; (rewrite length_make in C; [|math]).
-    { rewrite~ read_make. rewrite int_index_def. math. } 
-    { rewrite length_make; [|math]. math_rewrite (i-n = 0).
-      rewrite~ read_zero. } }
+    rewrite read_make; [| rewrite int_index_eq; math ].
+    rewrite read_app. rewrite length_make; [|math].
+    case_if as C.
+    { rewrite read_make. auto. rewrite int_index_eq; math. }
+    { math_rewrite (i-n = 0). rewrite~ read_zero. } }
 Qed.
 
-Lemma make_eq_cons_make_pred : forall n v, 
+Lemma make_eq_cons_make_pred : forall n v,
   0 < n -> 
-  v::(make (n - 1) v) = make n v.
+  make n v = v :: (make (n-1) v).
 Proof using.
-xxx reuse above
-  intros. unfold make.
-  do 2 (case_if; [ math | ]).
-  rewrite <- LibList.make_succ. fequals.
-  applys eq_nat_of_eq_int.
-  rewrite~ <- abs_eq_succ_abs_minus_one.
+  intros. math_rewrite (n = (n-1)+1). rewrite make_succ_l.
+  fequals_rec. math. math.
 Qed.
 
-End Make.
+End MakeNoInhab.
+
+Global Opaque make.
 
 
 (* ---------------------------------------------------------------------- *)
 (** * [LibList.map] interactions with [LibListZ] operations *)
 
-xx
+Section Map.
+Transparent index_inst read_inst update_inst.
+Context (A : Type).
+Implicit Types x v : A.
+Implicit Types l : list A.
+Implicit Types n i : int.
 
 Lemma length_map : forall A B (l:list A) (f:A->B),
   length (map f l) = length l.
@@ -508,7 +496,7 @@ Proof using. intros. unfold length. rewrite~ length_map. Qed.
 
 Lemma index_map_eq : forall A B (l:list A) i (f:A->B),
   index (map f l) i = index l i.
-Proof using. intros. rewrite index_def in *. rewrite~ length_map. Qed.
+Proof using. intros. rewrite index_eq_inbound in *. rewrite~ length_map. Qed.
 
 Lemma index_map : forall A B (l:list A) i (f:A->B),
   index l i -> index (map f l) i.
@@ -518,23 +506,25 @@ Lemma map_update : forall A B (l:list A) (i:int) (x:A) (f:A->B),
   index l i ->
   map f (l[i := x]) = (map f l)[i := f x].
 Proof using.
-  introv H. rewrite index_def, int_index_def in H.
+  introv H. rewrite index_eq_inbound in H.
   unfold update_inst, update_impl, update. simpl.
   case_if. { false; math. }
-  { applys list_update_map. { applys int_nat_lt. rewrite abs_pos; math. } }
+  { applys LibList.map_update. 
+    { applys lt_nat_of_lt_int. rewrite abs_nonneg; math. } }
 Qed.
 
 Lemma read_map : forall `{IA:Inhab A} `{IB:Inhab B} (l:list A) (i:int) (f:A->B),
   index l i ->
   (map f l)[i] = f (l[i]).
 Proof using.
-  introv H. rewrite index_def, int_index_def in H.
-  unfold read_inst, read_impl, nth. simpl. case_if.
+  introv H. rewrite index_eq_inbound in H.
+  unfold read_inst, read_impl. simpl. case_if.
   { false; math. }
-  { rewrite nth_map. (* TODO: why rewrite @nth_map fails *) auto.
-    applys int_nat_lt. rewrite abs_pos; math. }
+  { rewrite nth_map. auto.
+    applys lt_nat_of_lt_int. rewrite abs_nonneg; math. }
 Qed.
 
+End Map.
 
 
 (* ---------------------------------------------------------------------- *)
@@ -550,22 +540,6 @@ Instance card_inst : forall A, BagCard (list A).
 Proof using. constructor. rapply (@card_impl A). Defined.
 
 Global Opaque card_inst.
-
-
-(* ---------------------------------------------------------------------- *)
-(** * [binds], with length as [int], as typeclass *)
-
-(* --LATER: is this any useful?
-
-  Definition binds_impl A (l:list A) (i:int) (v:A) : Prop :=
-    index_impl l i /\ nth i l = v.
-
-  Instance binds_inst : forall A, BagBinds int A (list A).
-  Proof using. constructor. rapply (@binds_impl A). Defined.
-
-  Global Opaque binds_inst
-
-*)
 
 
 (* ---------------------------------------------------------------------- *)
@@ -628,3 +602,47 @@ Tactic Notation "rew_array" "*" "in" "*" :=
 (** Restore automation *)
 
 Ltac auto_tilde ::= auto_tilde_default.
+
+
+
+
+(* ********************************************************************** *)
+(** FUTURE WORK *)
+
+(*-- Lemmas on tail; is this useful? *)
+
+(*
+Lemma length_tail : forall l,
+  l <> nil -> 
+  length (tail l) = length l - 1.
+Proof using. induction l; intros; simpl; unfold length; rew_list. congruence. math. Qed.
+
+Lemma length_tail_le : forall l,
+  length (tail l) <= length l.
+Proof using. destruct l; simpl; unfold length; rew_list; math. Qed.
+
+Lemma length_le_1_inv_tail_eq_nil : forall l,
+  length l <= 1 -> 
+  tail l = nil.
+Proof using.
+  intros. destruct l; eauto.
+  simpl. unfold length in *. rew_list in *.
+  eapply length_zero_inv. math.
+Qed.
+*)
+
+
+(* ---------------------------------------------------------------------- *)
+(** * [binds], with length as [int], as typeclass *)
+
+(* --LATER: is this any useful?
+
+  Definition binds_impl A (l:list A) (i:int) (v:A) : Prop :=
+    index_impl l i /\ nth i l = v.
+
+  Instance binds_inst : forall A, BagBinds int A (list A).
+  Proof using. constructor. rapply (@binds_impl A). Defined.
+
+  Global Opaque binds_inst
+
+*)
